Denotational semantics written.

ecomp.v
@@ -1,5 +1,5 @@
 Require Import
-  Utf8.
+  Utf8 List String ListSet.
 
 (* Operators and expressions.  *)
 Inductive op : Set :=
@@ -8,13 +8,78 @@ Inductive op : Set :=
 
 Inductive expr : Set :=
   | num : nat → expr
+  | var : string → expr
   | biop : op → expr → expr → expr.
 
 Notation "x .+ y" := (biop add x y) (at level 50, left associativity).
 Notation "x .* y" := (biop mul x y) (at level 40, left associativity).
 Notation "[ x ]" := (num x).
 
-Example sample_expr := [3] .* [4] .+ [5] .* [9].
+Example sample_expr := [3] .* [4] .+ [5] .* ([9] .+ var "x").
+
+(* Variable bindings. *)
+
+Definition binds := list (string * nat).
+Notation "x ∪ y" := (set_union string_dec x y) (at level 50, left associativity).
+Notation "x ∈ S" := (set_In x S) (at level 30, no associativity).
+Notation "M ⊆ N" := (forall x, x ∈ M → x ∈ N) (at level 30, no associativity).
+Notation "f ∘ g" := (fun x => f (g x)) (at level 55, left associativity).
+
+Fixpoint freeVars (e : expr) : list string :=
+  match e with
+  | num _ => nil
+  | var v => v :: nil
+  | biop _ l r => freeVars l ∪ freeVars r
+  end.
+
+Definition boundVars : binds → list string := map (@fst _ _).
+
+Definition covered (bs : binds) (e : expr) := freeVars e ⊆ boundVars bs.
+
+Fixpoint lookup (v : string) (bs : binds) : option nat :=
+  match bs with
+  | nil => None
+  | (p,q) :: bs' => if string_dec p v then Some q else lookup v bs'
+  end.
+
+Lemma bound_weaken : forall s n v bs, s ≠ v → v ∈ boundVars ((s,n) :: bs) → v ∈ boundVars bs.
+  intros; induction bs.
+    simpl in H0; destruct H0; contradiction.
+    simpl in H0; destruct H0.
+      contradiction. destruct H0.
+      simpl; left; assumption.
+      simpl; right; assumption.
+Qed.
+
+Lemma lookup_pos : forall v bs, v ∈ boundVars bs → exists n, lookup v bs = Some n.
+  intros.
+  induction bs.
+    simpl in H; contradiction.
+    destruct a; simpl; destruct (string_dec s v).
+      exists n; reflexivity.
+      apply IHbs; apply (bound_weaken s n); assumption.
+Qed.
+
+Lemma lookup_pos_neg : forall v bs, v ∈ boundVars bs → lookup v bs ≠ None.
+  intros; destruct (lookup_pos _ _ H) as [n H0]; rewrite H0; discriminate.
+Qed.
+
+Program Definition slookup (v : string) (bs : binds) (pf : v ∈ boundVars bs) : nat :=
+  match lookup v bs with
+  | None => _
+  | Some x => x
+  end.
+Next Obligation.
+  destruct (lookup_pos_neg v bs pf (eq_sym Heq_anonymous)).
+Defined.
+
+Lemma expr_subvars_l : forall o l r, freeVars l ⊆ freeVars (biop o l r).
+  intros; simpl; apply set_union_intro1; assumption.
+Qed.
+
+Lemma expr_subvars_r : forall o l r, freeVars r ⊆ freeVars (biop o l r).
+  intros; simpl; apply set_union_intro2; assumption.
+Qed.
 
 (* Denotational semantics of ops and expressions. *)
 Definition d_op (o : op) : nat → nat → nat :=
@@ -23,18 +88,31 @@ Definition d_op (o : op) : nat → nat → nat :=
   | mul => mult
   end.
 
-Fixpoint denotation (e : expr) : nat :=
+Program Fixpoint denotation (e : expr) (bs : binds) (pf : freeVars e ⊆ boundVars bs) {struct e} : nat :=
   match e with
-  | num x => x
-  | biop o l r => d_op o (denotation l) (denotation r)
+  | num x => x 
+  | var v => slookup v bs _
+  | biop o l r => d_op o (denotation l bs _) (denotation r bs _)
   end.
+Next Obligation.
+  simpl in pf; exact (pf v (or_introl _ (eq_refl v))).
+Qed.
+Next Obligation.
+  apply pf; apply (expr_subvars_l o l r x H).
+Qed.
+Next Obligation.
+  apply pf; apply (expr_subvars_r o l r x H).
+Qed.
 
+(* Makes coqtop hang at this point:
 Eval compute in (denotation sample_expr).
+*)
 
 (* Instruction of a stack machine of type [instr s t] transforms
     a stack of size [s] into a stack of size [t]. *)
 Inductive instr : nat → nat → Set :=
   | ipush : forall {s}, nat → instr s (S s)
+  | iread : forall {s}, string → instr s (S s)
   | ibiop : forall {s}, op → instr (S (S s)) (S s).
 
 (* Code is a snoc-sequence of instructions, indexed by its action on stack. *)
@@ -48,12 +126,12 @@ Fixpoint cappend {s t u : nat} (p : code s t) (q : code t u) : code s u.
     assumption ||
     exact (csnoc (cappend s s0 t p q) i).
 Defined.
-Print cappend.
 
 (* Compilation of an expression into code. *)
 Fixpoint compile (e : expr) {s : nat} : code s (S s) :=
   match e with
   | num x => csnoc cnil (ipush x)
+  | var v => csnoc cnil (iread v)
   | biop o l r => csnoc (cappend (compile l) (compile r)) (ibiop o)
   end.
 
@@ -76,9 +154,10 @@ Definition exec_op (o : op) {s} (st : stack nat (S (S s))) : stack nat (S s) :=
   spush _ (d_op o x y) st''.
  
 (* Operational semantics of an instruction. *)
-Definition exec {s t} (i : instr s t) : stack nat s → stack nat t.
-  destruct i;
-    exact (spush _ n) ||
+Definition exec {s t} (i : instr s t) (bs : binds) : stack nat s → stack nat t.
+  destruct i.
+    exact (spush _ n).
+    exact (spush _ s0).
     exact (exec_op o).
 Defined.
 Print exec.    
